## 4.3 Writing a Grammar

### 4.3.1

> The following is a grammar for regular expressions over symbols $$a$$ and $$b$$ only, using `+` in place of `|` for union, to avoid conflict with the use of vertical bar as a metasymbol in grammars:

> $$
\begin{array}{lll}
rexpr &\rightarrow& rexpr~+~rterm~|~rterm \\
rterm &\rightarrow& rterm~rfactor~|~rfactor \\
rfactor &\rightarrow& rfactor~*~|~rprimary \\
rprimary &\rightarrow& \mathbf{a}~|~\mathbf{b} \\
\end{array}
$$

> a) Left factor this grammar.

No left factor.

> b) Dose left factoring make the grammar suitable for top-down parsing?

No.

> c) In addition to left factoring, eliminate left recursion from the original grammar.

$$
\begin{array}{lll}
rexpr &\rightarrow& rterm~rexpr' \\
rexpr' &\rightarrow& +~rexpr'~|~\epsilon \\
rterm &\rightarrow& rfactor~rterm' \\
rterm' &\rightarrow& rfactor~rterm'~|~\epsilon \\
rfactor &\rightarrow& rprimary~rfactor' \\
rfactor' &\rightarrow& *~rfactor'~|~\epsilon \\
rprimary &\rightarrow& \mathbf{a}~|~\mathbf{b} \\
\end{array}
$$

> d) Is the resulting grammar suitable for top-down parsing?

Yes.

[tool](https://cyberzhg.github.io/toolbox/cfg2ll?grammar=cmV4cHIgLT4gcmV4cHIgKyBydGVybSB8IHJ0ZXJtCnJ0ZXJtIC0+IHJ0ZXJtIHJmYWN0b3IgfCByZmFjdG9yCnJmYWN0b3IgLT4gcmZhY3RvciAqIHwgcnByaW1hcnkKcnByaW1hcnkgLT4gYSB8IGI=)

### 4.3.2

> Repeat Exercise 4.3.1 on the following grammars:

> a) The grammar of Exercise 4.2.1.

> $$
S~\rightarrow~S~S~+~|~S~S~*~|~a$$

Left factoring:

$$
\begin{array}{lcl}
S &\rightarrow& S~S~S'~|~a \\
S' &\rightarrow& +~|~* \\
\end{array}
$$

Left recursion:

$$
\begin{array}{lcl}
S &\rightarrow& a~S^{\prime\prime} \\
S^{\prime\prime} &\rightarrow& S~S^\prime~S^{\prime\prime}~|~\epsilon \\
S^\prime &\rightarrow& +~|~* \\
\end{array}
$$

[tool](https://cyberzhg.github.io/toolbox/cfg2ll.html?grammar=UyAtPiBTIFMgKyB8IFMgUyAqIHwgYQ==)

> b) The grammar of Exercise 4.2.2(a).

> $$
S~\rightarrow~0~S~1~|~0~1$$

Left factoring:

$$
\begin{array}{lcl}
S &\rightarrow& 0~S' \\
S' &\rightarrow& S~1~|~1 \\
\end{array}
$$

Left recursion:

$$
\begin{array}{lcl}
S &\rightarrow& 0~S' \\
S' &\rightarrow& 0~S'~1~|~1 \\
\end{array}
$$

[tool](https://cyberzhg.github.io/toolbox/cfg2ll.html?grammar=UyAtPiAwIFMgMSB8IDAgMQ==)

> c) The grammar of Exercise 4.2.2(c).

> $$
S~\rightarrow~S~(~S~)~S~|~\epsilon$$

Left recursion:

$$
\begin{array}{lcl}
S &\rightarrow& (~S~)~S~S~|~\epsilon \\
\end{array}
$$

[tool](https://cyberzhg.github.io/toolbox/cfg2ll?grammar=UyAtPiBTICggUyApIFMgfCDPtQ==)

> d) The grammar of Exercise 4.2.2(e).

> $$
\begin{array}{lll}
S &\rightarrow& (~L~)~|~a \\
L &\rightarrow& L~,~S~|~S~ \\
\end{array}$$

Left recursion:

$$
\begin{array}{lcl}
S &\rightarrow& (~L~)~|~a \\
L &\rightarrow& (~L~)~L'~|~a~L' \\
L' &\rightarrow& ,~S~L'~|~\epsilon \\
\end{array}
$$

[tool](https://cyberzhg.github.io/toolbox/cfg2ll?grammar=UyAtPiAoIEwgKSB8IGEgTCAtPiBMICwgUyB8IFM=)

> e) The grammar of Exercise 4.2.2(g).

> $$
\begin{array}{lll}
bexpr &\rightarrow& bexpr~\mathbf{or}~bterm~|~bterm \\
bterm &\rightarrow& bterm~\mathbf{and}~bfactor~|~bfactor \\
bfactor &\rightarrow& \mathbf{not}~bfactor~|~(~bexpr~)~|~\mathbf{true}~|~\mathbf{false} \\
\end{array}
$$

Left recursion:

$$
\begin{array}{lcl}
bexpr &\rightarrow& bterm~bexpr' \\
bexpr' &\rightarrow& \mathbf{or}~bterm~bexpr'~|~\epsilon \\
bterm &\rightarrow& bfactor~bterm' \\
bterm' &\rightarrow& \mathbf{and}~bfactor~bterm'~|~\epsilon \\
bfactor &\rightarrow& \mathbf{not}~bfactor~|~(~bexpr~)~|~\mathbf{true}~|~\mathbf{false} \\
\end{array}
$$

[tool](https://cyberzhg.github.io/toolbox/cfg2ll?grammar=YmV4cHIgLT4gYmV4cHIgb3IgYnRlcm0gfCBidGVybSAKYnRlcm0gLT4gYnRlcm0gYW5kIGJmYWN0b3IgfCBiZmFjdG9yIApiZmFjdG9yIC0+IG5vdCBiZmFjdG9yIHwgKCBiZXhwciApIHwgdHJ1ZSB8IGZhbHNl)

### 4.3.3

> The following grammar is proposed to remove the "dangling-else ambiguity" discussed in Section 4.3.2:

> $$
\begin{array}{lcl}
stmt &\rightarrow& \mathbf{if}~expr~\mathbf{then}~stmt \\
&|& matchedStmt \\
matchedStmt &\rightarrow& \mathbf{if}~expr~\mathbf{then}~matchedStmt~\mathbf{else}~stmt \\
&|& \mathbf{other} \\
\end{array}
$$

> Show that this grammar is still ambiguous.

$$\mathbf{if}~A~\mathbf{then}~\mathbf{if}~B~\mathbf{then}~\mathbf{if}~C~\mathbf{then}~D~\mathbf{else}~E~\mathbf{else}~F$$

```
if A
then
    if B
    then
        if C
        then D
    else E
else F
```

```
if A
then
    if B
    then
        if C
        then D
        else E
    else F
```
