
### 4.4.2

> Is it possible, by modifying the grammar in any way, to construct a predictive parser for the language of Exercise 4.2.1 (postfix expressions with oprand $$a$$)?

> $$ S~\rightarrow~S~S~+~|~S~S~*~|~a$$

$$\begin{array}{lcl}
S &\rightarrow& a~S^{\prime\prime} \\
S^{\prime\prime} &\rightarrow& S~S^\prime~S^{\prime\prime}~|~\epsilon \\
S^\prime &\rightarrow& +~|~* \\
\end{array}$$

| NON-TERMINAL | $$+$$ | $$*$$ | $$a$$ | $$\$$$ |
|:------------:|:-:|:-:|:-:|:-:|
|$$S$$|$$~$$|$$~$$|$$S \rightarrow a~S^{\prime\prime}$$|$$~$$|
|$$S^\prime$$|$$S^\prime \rightarrow +$$|$$S^\prime \rightarrow *$$|$$~$$|$$~$$|
|$$S^{\prime\prime}$$|$$S^{\prime\prime} \rightarrow \epsilon$$|$$S^{\prime\prime} \rightarrow \epsilon$$|$$S^{\prime\prime} \rightarrow S~S^\prime~S^{\prime\prime}$$|$$S^{\prime\prime} \rightarrow \epsilon$$|

### 4.4.3

> Compute FIRST and FOLLOW for the grammar of Exercise 4.2.1.

FIRST($$S$$) = $$\{ a \}$$

FOLLOW($$S$$) = $$\{ +, *, a \}$$

### 4.4.4

> Compute FIRST and FOLLOW for each of the grammars of Exercise 4.2.2.

> a) $$S~\rightarrow~0~S~1~|~0~1$$.

FIRST($$S$$) = $$\{ 0 \}$$

FOLLOW($$S$$) = $$\{ 1, $ \}$$

> b) $$S~\rightarrow~+~S~S~|~*~S~S~|~a$$.

FIRST($$S$$) = $$\{ +, *, a \}$$

FOLLOW($$S$$) = $$\{ +, *, a, $ \}$$

> c) $$S~\rightarrow~S~(~S~)~S~|~\epsilon$$.

FIRST($$S$$) = $$\{ (, \epsilon \}$$

FOLLOW($$S$$) = $$\{ (, ), $ \}$$

> d) $$S~\rightarrow~S~+~S~|~S~S~|~(~S~)|~S~*~|~a$$.

FIRST($$S$$) = $$\{ (, a \}$$

FOLLOW($$S$$) = $$\{ +, (, ), *, a, $ \}$$

> e) $$S~\rightarrow~(~L~)~|~a$$ and $$L~\rightarrow~L~,~S~|~S~$$.

FIRST($$S$$) = $$\{ (, a \}$$

FOLLOW($$S$$) = $$\{ ',', ), $ \}$$

FIRST($$L$$) = $$\{ (, a \}$$

FOLLOW($$L$$) = $$\{ ',', ) \}$$

> f) $$S~\rightarrow~a~S~b~S~|~b~S~a~S~|~\epsilon$$.

FIRST($$S$$) = $$\{ a, b, \epsilon \}$$

FOLLOW($$S$$) = $$\{ a, b, $ \}$$

> g) The following grammar for boolean expressions:

> $$
\begin{array}{rll}
bexpr &\rightarrow& bexpr~\mathbf{or}~bterm~|~bterm \\
bterm &\rightarrow& bterm~\mathbf{and}~bfactor~|~bfactor \\
bfactor &\rightarrow& \mathbf{not}~bfactor~|~(~bexpr~)~|~\mathbf{true}~|~\mathbf{false} \\
\end{array}
$$

FIRST($$bfactor$$) = $$\{ \mathbf{not}, (, \mathbf{true}, \mathbf{false} \}$$

FOLLOW($$bfactor$$) = $$\{ ), \mathbf{and}, \mathbf{or}, $ \}$$

FIRST($$bterm$$) = $$\{ \mathbf{not}, (, \mathbf{true}, \mathbf{false} \}$$

FOLLOW($$bterm$$) = $$\{ ), \mathbf{and}, $ \}$$

FIRST($$bexpr$$) = $$\{ \mathbf{not}, (, \mathbf{true}, \mathbf{false} \}$$

FOLLOW($$bexpr$$) = $$\{ ), \mathbf{or}, $ \}$$

### 4.4.5

> The grammar $$S~\rightarrow~a~S~a~|~a~a$$ generates all even-length strings of $$a$$'s. We can devise a recursive-descent parser with backtrack for this grammar. If we choose to expand by production $$S~\rightarrow~a~a$$ first, then we shall only recognize the string $$aa$$. Thus, any reasonable recursive-descent parser will try $$S~\rightarrow~a~S~a$$ first.

> a) Show that this recursive-descent parser recognizes input $$aa$$, $$aaaa$$, and $$aaaaaaaa$$, but not $$aaaaaa$$.

> b) What language does this recursive-descent parser recognize?

$$2^n$$ $$a$$s.
