## 4.4 Top-Down Parsing

### 4.4.1

> For each of the following grammars, devise predictive parsers and show the parsing tables. You may left-factor and/or eliminate left-recursion from your grammars first.

> a) The grammar of Exercise 4.2.2(a).

> $$ S~\rightarrow~0~S~1~|~0~1$$

$$\begin{array}{lcl}
S &\rightarrow& 0~S' \\
S' &\rightarrow& S~1~|~1 \\
\end{array}$$

| NON-TERMINAL | $$0$$ | $$1$$ | $$\$$$ |
|:------------:|:-:|:-:|:-:|
| $$S$$ | $$S \rightarrow 0~S'$$|  |  |
| $$S'$$ | $$S' \rightarrow S~1$$ | $$S' \rightarrow 1$$ |  |

> b) The grammar of Exercise 4.2.2(b).

> $$S~\rightarrow~+~S~S~|~*~S~S~|~a$$

| NON-TERMINAL | $$+$$ | $$*$$ | $$a$$ | $$\$$$ |
|:------------:|:-:|:-:|:-:|:-:|
| $$S$$ | $$S \rightarrow +~S~S$$| $$S \rightarrow *~S~S$$ | $$S \rightarrow a$$ |   |

> c) The grammar of Exercise 4.2.2(c).

> $$S~\rightarrow~S~(~S~)~S~|~\epsilon$$

$$\begin{array}{lcl}
S &\rightarrow& (~S~)~S~S~|~\epsilon \\
\end{array}$$

| NON-TERMINAL | $$($$ | $$)$$ | $$\$$$ |
|:------------:|:-:|:-:|:-:|
| $$S$$ | $$S \rightarrow (~S~)~S~S$$| $$S \rightarrow \epsilon$$ | $$S \rightarrow \epsilon$$ |

> d) The grammar of Exercise 4.2.2(d).

> $$S~\rightarrow~S~+~S~|~S~S~|~(~S~)|~S~*~|~a$$

Left factoring:

$$\begin{array}{lcl}
S &\rightarrow& S~S'~|~(~S~)|~a \\
S' &\rightarrow& +~S~|~S~|~*~ \\
\end{array}$$

Left recursion:

$$\begin{array}{lcl}
S &\rightarrow& (~S~)~S^{\prime\prime}~|~a~S^{\prime\prime} \\
S' &\rightarrow& +~S~|~S~|~*~ \\
S^{\prime\prime} &\rightarrow& S'~S^{\prime\prime}~|~\epsilon \\
\end{array}$$

| NON-TERMINAL | $$($$ | $$)$$ | $$+$$ | $$*$$ | $$a$$ | $$\$$$ |
|:------------:|:-:|:-:|:-:|:-:|:-:|:-:|
| $$S$$ | $$S \rightarrow (~S~)~S^{\prime\prime}$$ |   |   |   | $$S \rightarrow a~S^{\prime\prime}$$ |   |
| $$S^{\prime}$$ | $$S^{\prime} \rightarrow S$$ |   | $$S^{\prime} \rightarrow +~S$$ | $$S^{\prime} \rightarrow *$$ | $$S^{\prime} \rightarrow S$$ |   |
| $$S^{\prime\prime}$$ | $$S^{\prime\prime} \rightarrow S'S^{\prime\prime}$$ |   | $$S^{\prime\prime} \rightarrow S'S^{\prime\prime}$$ | $$S^{\prime\prime} \rightarrow S'S^{\prime\prime}$$ | $$S^{\prime\prime} \rightarrow S'S^{\prime\prime}$$ | $$S^{\prime\prime} \rightarrow \epsilon$$ |

> e) The grammar of Exercise 4.2.2(e).

> $$\begin{array}{lll}
S &\rightarrow& (~L~)~|~a \\
L &\rightarrow& L~,~S~|~S~ \\
\end{array}$$

$$\begin{array}{lcl}
S &\rightarrow& (~L~)~|~a \\
L &\rightarrow& S~L' \\
L' &\rightarrow& ,~S~L'~|~\epsilon \\
\end{array}$$

| NON-TERMINAL | $$($$ | $$)$$ | $$,$$ | $$a$$ | $$\$$$ |
|:------------:|:-:|:-:|:-:|:-:|:-:|
| $$S$$ | $$S \rightarrow (~L~)~$$ |   |   | $$S \rightarrow a$$ |   |
| $$L$$ | $$L \rightarrow S~L'$$ |   |   | $$L \rightarrow S~L'$$ |   |
| $$L'$$ |   |   | $$L' \rightarrow ,~S~L'$$ |   | $$L' \rightarrow \epsilon$$ |

> f) The grammar of Exercise 4.2.2(g).

> $$\begin{array}{lll}
bexpr &\rightarrow& bexpr~\mathbf{or}~bterm~|~bterm \\
bterm &\rightarrow& bterm~\mathbf{and}~bfactor~|~bfactor \\
bfactor &\rightarrow& \mathbf{not}~bfactor~|~(~bexpr~)~|~\mathbf{true}~|~\mathbf{false} \\
\end{array}$$

$$\begin{array}{lcl}
bexpr &\rightarrow& bterm~bexpr' \\
bexpr' &\rightarrow& \mathbf{or}~bterm~bexpr'~|~\epsilon \\
bterm &\rightarrow& bfactor~bterm' \\
bterm' &\rightarrow& \mathbf{and}~bfactor~bterm'~|~\epsilon \\
bfactor &\rightarrow& \mathbf{not}~bfactor~|~(~bexpr~)~|~\mathbf{true}~|~\mathbf{false} \\
\end{array}$$

| NON-TERMINAL | $$\mathbf{and}$$ | $$\mathbf{or}$$ | $$\mathbf{not}$$ | $$($$ | $$)$$ | $$\mathbf{true}$$ | $$\mathbf{false}$$ | $$\$$$ |
|:------------:|:-:|:-:|:-:|:-:|:-:|:-:|:-:|:-:|
| $$bexpr$$ |   |   | $$bexpr \rightarrow bterm~bexpr'$$ | $$bexpr \rightarrow bterm~bexpr'$$ |   | $$bexpr \rightarrow bterm~bexpr'$$ | $$bexpr \rightarrow bterm~bexpr'$$ |   |
| $$bexpr'$$ |   | $$bexpr' \rightarrow \mathbf{or}~bterm~bexpr'$$ |   |   | $$bexpr' \rightarrow \epsilon$$ |   |   | $$bexpr' \rightarrow \epsilon$$ |
| $$bterm$$ |   |   | $$bterm \rightarrow bfactor~bterm'$$ | $$bterm \rightarrow bfactor~bterm'$$ |   | $$bterm \rightarrow bfactor~bterm'$$ | $$bterm \rightarrow bfactor~bterm'$$ |   |
| $$bterm'$$ | $$bterm' \rightarrow \mathbf{and}~bfactor~bterm'$$ |   |   |   | $$bterm' \rightarrow \epsilon$$ |   |   | $$bterm' \rightarrow \epsilon$$ |
| $$bfactor$$ |   |   | $$bfactor \rightarrow \mathbf{not}~bfactor$$ | $$bfactor \rightarrow (~bexpr~)$$ |   | $$bfactor \rightarrow \mathbf{true}$$ | $$bfactor \rightarrow \mathbf{false}$$ |   |


### 4.4.2

> Is it possible, by modifying the grammar in any way, to construct a predictive parser for the language of Exercise 4.2.1 (postfix expressions with oprand $$a$$)?

> $$ S~\rightarrow~S~S~+~|~S~S~*~|~a$$

$$\begin{array}{lcl}
S &\rightarrow& a~S^{\prime\prime} \\
S^{\prime\prime} &\rightarrow& S~S^\prime~S^{\prime\prime}~|~\epsilon \\
S^\prime &\rightarrow& +~|~* \\
\end{array}$$

| NON-TERMINAL | $$+$$ | $$*$$ | $$a$$ | $$\$$$ |
|:------------:|:-:|:-:|:-:|:-:|
|$$S$$|$$~$$|$$~$$|$$S \rightarrow a~S^{\prime\prime}$$|$$~$$|
|$$S^\prime$$|$$S^\prime \rightarrow +$$|$$S^\prime \rightarrow *$$|$$~$$|$$~$$|
|$$S^{\prime\prime}$$|$$S^{\prime\prime} \rightarrow \epsilon$$|$$S^{\prime\prime} \rightarrow \epsilon$$|$$S^{\prime\prime} \rightarrow S~S^\prime~S^{\prime\prime}$$|$$S^{\prime\prime} \rightarrow \epsilon$$|

### 4.4.3

> Compute FIRST and FOLLOW for the grammar of Exercise 4.2.1.

FIRST($$S$$) = $$\{ a \}$$

FOLLOW($$S$$) = $$\{ +, *, a \}$$

### 4.4.4

> Compute FIRST and FOLLOW for each of the grammars of Exercise 4.2.2.

> a) $$S~\rightarrow~0~S~1~|~0~1$$.

FIRST($$S$$) = $$\{ 0 \}$$

FOLLOW($$S$$) = $$\{ 1, $ \}$$

> b) $$S~\rightarrow~+~S~S~|~*~S~S~|~a$$.

FIRST($$S$$) = $$\{ +, *, a \}$$

FOLLOW($$S$$) = $$\{ +, *, a, $ \}$$

> c) $$S~\rightarrow~S~(~S~)~S~|~\epsilon$$.

FIRST($$S$$) = $$\{ (, \epsilon \}$$

FOLLOW($$S$$) = $$\{ (, ), $ \}$$

> d) $$S~\rightarrow~S~+~S~|~S~S~|~(~S~)|~S~*~|~a$$.

FIRST($$S$$) = $$\{ (, a \}$$

FOLLOW($$S$$) = $$\{ +, (, ), *, a, $ \}$$

> e) $$S~\rightarrow~(~L~)~|~a$$ and $$L~\rightarrow~L~,~S~|~S~$$.

FIRST($$S$$) = $$\{ (, a \}$$

FOLLOW($$S$$) = $$\{ ',', ), $ \}$$

FIRST($$L$$) = $$\{ (, a \}$$

FOLLOW($$L$$) = $$\{ ',', ) \}$$

> f) $$S~\rightarrow~a~S~b~S~|~b~S~a~S~|~\epsilon$$.

FIRST($$S$$) = $$\{ a, b, \epsilon \}$$

FOLLOW($$S$$) = $$\{ a, b, $ \}$$

> g) The following grammar for boolean expressions:

> $$
\begin{array}{rll}
bexpr &\rightarrow& bexpr~\mathbf{or}~bterm~|~bterm \\
bterm &\rightarrow& bterm~\mathbf{and}~bfactor~|~bfactor \\
bfactor &\rightarrow& \mathbf{not}~bfactor~|~(~bexpr~)~|~\mathbf{true}~|~\mathbf{false} \\
\end{array}
$$

FIRST($$bfactor$$) = $$\{ \mathbf{not}, (, \mathbf{true}, \mathbf{false} \}$$

FOLLOW($$bfactor$$) = $$\{ ), \mathbf{and}, \mathbf{or}, $ \}$$

FIRST($$bterm$$) = $$\{ \mathbf{not}, (, \mathbf{true}, \mathbf{false} \}$$

FOLLOW($$bterm$$) = $$\{ ), \mathbf{and}, $ \}$$

FIRST($$bexpr$$) = $$\{ \mathbf{not}, (, \mathbf{true}, \mathbf{false} \}$$

FOLLOW($$bexpr$$) = $$\{ ), \mathbf{or}, $ \}$$

### 4.4.5

> The grammar $$S~\rightarrow~a~S~a~|~a~a$$ generates all even-length strings of $$a$$'s. We can devise a recursive-descent parser with backtrack for this grammar. If we choose to expand by production $$S~\rightarrow~a~a$$ first, then we shall only recognize the string $$aa$$. Thus, any reasonable recursive-descent parser will try $$S~\rightarrow~a~S~a$$ first.

> a) Show that this recursive-descent parser recognizes input $$aa$$, $$aaaa$$, and $$aaaaaaaa$$, but not $$aaaaaa$$.

> b) What language does this recursive-descent parser recognize?

$$2^n$$ $$a$$s.

### 4.4.6

> A grammar is $$\epsilon$$-_free_ if no production body is $$\epsilon$$ (called an $$\epsilon$$-_production_).

> a) Give an algorithm to convert any grammar into an $$\epsilon$$-free grammar that generates the same language.

Find all nullables in a production, enumerate all the situations that each nullable appears or not.

> b) Apply your algorithm to the grammar $$S~\rightarrow~a~S~b~S~|~b~S~a~S~|~\epsilon$$.

$$\begin{array}{lcl}
S &\rightarrow& a~S~b~S \\
&|& a~S~b \\
&|& a~b~S \\
&|& a~b \\
&|& b~S~a~S \\
&|& b~S~a \\
&|& b~a~S \\
&|& b~a \\
\end{array}$$

### 4.4.7

> A _single production_ is a production whose body is a single nonterminal, i.e., a production of the form $$A \rightarrow B$$.

> a) Give an algorithm to convert any grammar into a $$\epsilon$$-free grammar, with no single productions, that generate the same language.

If $$A \Rightarrow B$$, replace $$A$$ with $$B$$.

> b) Apply your algorithm to the grammar (4.1) in Section 4.1.2.

> $$\begin{array}{lcl}
E &\rightarrow& E~+~T~|~T \\
T &\rightarrow& T~*~F~|~F \\
F &\rightarrow& (~E~)~|~\mathbf{id} \\
\end{array}$$

$$\begin{array}{lcl}
E &\rightarrow& E~+~T~|~T~*~F~|~(~E~)~|~\mathbf{id} \\
T &\rightarrow& T~*~F~|~(~E~)~|~\mathbf{id} \\
\end{array}$$

> c) Show that, as a consequence of part (a), we can convert a grammar into an equivalent grammar that has no _cycles_.
