## 5.3 Applications of Syntax-Directed Translation

### 5.3.1

> Below is a grammar for expressions involving operation $$+$$ and integer or floating-point operands. Floating-point numbers are distinguished by having a decimal point.

> $$
\begin{array}{rll}
E &\rightarrow& E~+~T~|~T \\
T &\rightarrow& \mathbf{num}~.~\mathbf{num}~|~\mathbf{num}
\end{array}
$$

> a) Give an SDD to determine the type of each Term $$T$$ and expression $$E$$.

|    | Production | Semantic Rules |
|:--:|:-----------|:---------------|
| 1) | $$E~\rightarrow~E_1~+~T$$ | $$\mathbf{if}~E_1.t = integer~\mathbf{and}~T.t=integer \\ \mathbf{then}~E.t = integer \\ \mathbf{else}~E.t = float$$ |
| 2) | $$E~\rightarrow~T$$ | $$E.t = T.t$$ |
| 3) | $$T~\rightarrow~\mathbf{num}~.~\mathbf{num}$$ | $$T.t = float$$ |
| 4) | $$T~\rightarrow~\mathbf{num}$$ | $$T.t = integer$$ |

> b) Extend your SDD of (a) to translate expressions into postfix notation. Use the unary operator __intToFloat__ to turn an integer into an equivalent float.

|    | Production | Semantic Rules |
|:--:|:-----------|:---------------|
| 1) | $$E~\rightarrow~E_1~+~T$$ | $$\mathbf{if}~E_1.t = integer~\mathbf{and}~T.t=integer \\~~~~E.t = integer \\~~~~E.lex = E_1.lex + "~" + T.lex + "+"\\ \mathbf{else~if}~E_1.t = integer~\mathbf{and}~T.t=float \\~~~~E.t = float \\~~~~E.lex = E_1.lex + "~\mathbf{intToFloat}~" + T.lex + "+" \\ \mathbf{else~if}~E_1.t = float~\mathbf{and}~T.t=integer \\~~~~E.t = float \\~~~~E.lex = E_1.lex + " " + T.lex +  "~\mathbf{intToFloat}~" + "+" \\ \mathbf{else} \\
~~~~E.t = float \\~~~~E.lex = E_1.lex + "~" + T.lex + "+"$$ |
| 2) | $$E~\rightarrow~T$$ | $$E.t = T.t \\ E.lex = T.lex$$ |
| 3) | $$T~\rightarrow~\mathbf{num}_1~.~\mathbf{num}_2$$ | $$T.t = float \\ T.lex = \mathbf{num}_1.lexval + "." + \mathbf{num}_2.lexval $$ |
| 4) | $$T~\rightarrow~\mathbf{num}$$ | $$T.t = integer \\ T.lex = \mathbf{num}.lexval$$ |

### 5.3.2

> Give an SDD to translate infix expressions with $$+$$ and $$*$$ into equivalent expressions without redundant parentheses. For example, since both operators associate form the left, and $$*$$ takes precedence over $$+$$, $$((a*(b+c))*(d))$$ translates into $$a*(b+c)*d$$.

|    | Production | Semantic Rules |
|:---|:-----------|:-----                     ----------|
| 1) | $$L~\rightarrow~E~\mathbf{n}$$ | $$L.lex = E.lex$$ |
| 2) | $$E~\rightarrow~E_1~+~T$$ | $$E.lex = E_1.lex + `+` + T.lex\\ E.plus = \mathbf{true}$$ |
| 3) | $$E~\rightarrow~T$$ | $$E.lex = T.lex\\ E.plus = T.plus$$ |
| 4) | $$T~\rightarrow~T_1~*~F$$ | $$\mathbf{if}~T_1.plus~\\ \mathbf{then}~T.lex = `(` + T_1.lex + `)`\\ \mathbf{else}~T.lex=T_1.lex\\ T.lex += `*`\\ \mathbf{if}~F.plus~\\ \mathbf{then}~T.lex += `(` + F.lex + `)`\\ \mathbf{else}~T.lex+=F.lex\\ T.plus=\mathbf{false} $$ |
| 5) | $$T~\rightarrow~F$$ | $$T.lex = F.lex\\ T.plus = F.plus$$ |
| 6) | $$F~\rightarrow~(~E~)$$ | $$T.lex = E.lex\\ T.plus = E.plus$$ |
| 7) | $$F~\rightarrow~\mathbf{id}$$ | $$T.lex = \mathbf{id}.lex\\ T.plus = \mathbf{false}$$ |

### 5.3.3

> Given an SDD to differentiate expressions such as $$x*(3*x+x*x)$$ involving the operators $$+$$ and $$*$$, the variable $$x$$, and constants. Assume that no simplification occurs, so that, for examle, $$3*x$$ will be translated into $$3*1+0*x$$.

|    | Production | Semantic Rules |
|:---|:-----------|:-----                     ----------|
| 1) | $$L~\rightarrow~E~\mathbf{n}$$ | $$L.diff = E.diff $$ |
| 2) | $$E~\rightarrow~E_1~+~T$$ | $$E.lex = E_1.lex + `+` + T.lex\\ E.diff = E_1.diff + `+` + T.diff $$ |
| 3) | $$E~\rightarrow~T$$ | $$E.lex = T.lex \\ E.diff = T.diff $$ |
| 4) | $$T~\rightarrow~T_1~*~F$$ | $$T.lex = T_1.lex + `*` + F.lex\\ T.diff = T_1.lex + `*` + F.diff + `+` + T_1.diff + `*` + F.lex $$ |
| 5) | $$T~\rightarrow~F$$ | $$T.lex = F.lex\\ T.diff = F.diff $$ |
| 6) | $$F~\rightarrow~(~E~)$$ | $$F.lex = `(` + E.lex + `)`\\F.diff = `(` + E.diff + `)` $$ |
| 7) | $$F~\rightarrow~\mathbf{id}$$ | $$F.lex = \mathbf{id}.lexval\\ F.diff = 1 $$ | 
| 8) | $$F~\rightarrow~\mathbf{digit}$$ | $$F.lex = \mathbf{digit}.lexval\\ F.diff = 0 $$ | 
