## 6.4 Translation of Expressions

### 6.4.1

> Add to the translation of Fig. 6.19 rules for the following productions:

> a) $$E~\rightarrow~E_1~*~E_2$$.

> b) $$E~\rightarrow~+~E_1$$.

| PRODUCTION | SEMANTIC RULES |
|:-----------|:---------------|
|$$S\rightarrow\mathbf{id}=E;$$|$$\begin{array}{ll}S.code =&E.code~||~\\ &gen(top.get(\mathbf{id}.lexeme)~'='~E.addr)\end{array}$$|
|$$E\rightarrow E_1+E_2$$|$$\begin{array}{ll}E.addr =& \mathbf{new}~Temp()\\ E.code =& E_1.code~||~E_2.code~||~\\&gen(E.addr~'='~E_1.addr~'+'~E_2.addr)\end{array}$$|
|$$E\rightarrow E_1*E_2$$|$$\begin{array}{ll}E.addr =& \mathbf{new}~Temp()\\ E.code =& E_1.code~||~E_2.code~||~\\&gen(E.addr~'='~E_1.addr~'*'~E_2.addr)\end{array}$$|
|$$~~|+E_1$$|$$\begin{array}{ll}E.addr =& E_1.addr\\ E.code =& E_1.code\end{array}$$|
|$$~~|-E_1$$|$$\begin{array}{ll}E.addr =& \mathbf{new}~Temp()\\ E.code =& E_1.code~||~\\&gen(E.addr~'='~'\mathbf{minus}'~E_1.addr)\end{array}$$|
|$$~~(E_1)$$|$$\begin{array}{ll}E.addr=&E_1.addr\\E.code=&E_1.code\end{array}$$|
|$$~~\mathbf{id}$$|$$\begin{array}{ll}E.addr=&top.get(\mathbf{id}.lexeme)\\ E.code =& ''\end{array}$$

> b) $$E~\rightarrow~+~E_1$$.
