## 6.7 Backpatching

### 6.7.1

> Using the translation of Fig. 6.43, translate each of the following expressions. Show the true and false lists for each subexpression. You may assume the address of the first instruction generated is 100.

> a) `a==b && (c==d || e==f)`

| Expressions | True & false lists |
|:------------|:-------------------|
| `a==b` | $$\begin{array}{l}B.t = \{100\} \\B.f = \{101\} \end{array}$$ |
| `c==d` | $$\begin{array}{l}B.t = \{102\} \\B.f = \{103\} \end{array}$$ |
| `e==f` | $$\begin{array}{l}B.t = \{104\} \\B.f = \{105\} \end{array}$$ |
| `(c==d \|\| e==f)` | $$\begin{array}{l}B.t = \{102, 104\} \\B.f = \{105\} \end{array}$$ |
| `a==b && (c==d \|\| e==f)` | $$\begin{array}{l}B.t = \{102, 104\} \\B.f = \{101, 105\} \end{array}$$ |

> b) `(a==b || c==d) || e==f`

| Expressions | True & false lists |
|:------------|:-------------------|
| `a==b` | $$\begin{array}{l}B.t = \{100\} \\B.f = \{101\} \end{array}$$ |
| `c==d` | $$\begin{array}{l}B.t = \{102\} \\B.f = \{103\} \end{array}$$ |
| `(a==b \|\| c==d)` | $$\begin{array}{l}B.t = \{100, 102\} \\B.f = \{103\} \end{array}$$ |
| `e==f` | $$\begin{array}{l}B.t = \{104\} \\B.f = \{105\} \end{array}$$ |
| `(a==b \|\| c==d) \|\| e==f` | $$\begin{array}{l}B.t = \{100, 102, 104\} \\B.f = \{105\} \end{array}$$ |

> c) `(a==b && c==d) && e==f`

| Expressions | True & false lists |
|:------------|:-------------------|
| `a==b` | $$\begin{array}{l}B.t = \{100\} \\B.f = \{101\} \end{array}$$ |
| `c==d` | $$\begin{array}{l}B.t = \{102\} \\B.f = \{103\} \end{array}$$ |
| `(a==b && c==d)` | $$\begin{array}{l}B.t = \{102\} \\B.f = \{101, 103\} \end{array}$$ |
| `e==f` | $$\begin{array}{l}B.t = \{104\} \\B.f = \{105\} \end{array}$$ |
| `(a==b && c==d) && e==f` | $$\begin{array}{l}B.t = \{104\} \\B.f = \{101, 104, 105\} \end{array}$$ |

### 6.7.2

> Give the value that eventually replaces each place on each of the following lists:

> (a) $$B_3.false$$ (b) $$S_2.next$$ (c) $$B_4.false$$ (d) $$S_1.next$$ (e) $$B_2.true$$

* $$B_3.false = i_1$$
* $$S_2.next = i_7$$
* $$B_4.false = i_7$$
* $$S_1.next = i_3$$
* $$B_2.true = i_3$$

### 6.7.3

> Give the rules for

> (a) $$S_4.next$$ (b) $$S_5.next$$ (c) $$S_6.next$$ (d) $$S_7.next$$ (e) $$S_8.next$$

* $$S_4.next = B_3.false$$
* $$S_5.next = merge(B_4.false, S_2.next)$$
* $$S_6.next = S_3.next$$
* $$S_7.next = merge(S_4.next, N.next, S_6.next)$$
* $$S_8.next = B_1.false$$
