> (fib/k n g) = (g (fib n))

```
(define fib
  (lambda (n)
    (fib/k n (lambda (val) val))))

(define fib/k
  (lambda (n cont)
    (if (< n 2)
        (cont 1)
        (fib/k (- n 1)
               (lambda (val1)
                 (fib/k (- n 2)
                        (lambda (val2)
                          (cont (+ val1 val2)))))))))
```

`(fib/k 0 g) = (g 1) = (g (fib 0))`

`(fib/k 1 g) = (g 1) = (g (fib 1))`

Assume that `n >= 2`, `(fib/k (n - 1) g) = (g (fib (n - 1)))` and `(fib/k (n - 2) g) = (g (fib (n - 2)))`.

  (fib/k n g) = (fib/k (n - 1) (lambda (val1) (fib/k (n - 2) (lambda (val2) (g (val1 + val2))))))

= ((lambda (val1) (fib/k (n - 2) (lambda (val2) (g (val1 + val2))))) (fib (n - 1)))

= (fib/k (n - 2) (lambda (val2) (g ((fib (n - 1)) + val2))))

= ((lambda (val2) (g ((fib (n - 1)) + val2))) (fib (n - 2)))

= (g ((fib (n - 1)) + (fib (n - 2))))

= (g (fib n))
