```
                       (value-of exp1 ρ σ0) = (val1, σ1)
                       (value-of exp2 ρ σ1) = (val2, σ2)
--------------------------------------------------------------------------------
(value-of (newpair-exp exp1 exp2) ρ σ0) = ((a-pair f1 f2), [f1=val1, f2=val2]σ2)
```

```
(value-of (left-exp (a-pair ref1 ref2)) ρ σ) = (σ(ref1), σ)
```

```
(value-of (right-exp (a-pair ref1 ref2)) ρ σ) = (σ(ref2), σ)
```

```
                             (value-of exp2 ρ σ0) = (val2, σ2)
-------------------------------------------------------------------------------------------
(value-of (setleft-exp (a-pair ref1 ref2) exp2) ρ σ0) = ((a-pair ref1 ref2), [ref1=val2]σ2)
```

```
                             (value-of exp2 ρ σ0) = (val2, σ2)
-------------------------------------------------------------------------------------------
(value-of (setleft-exp (a-pair ref1 ref2) exp2) ρ σ0) = ((a-pair ref1 ref2), [ref2=val2]σ2)
```
